src/Init/Data/Iterators/Combinators/Monadic/ULift.lean
@@ -140,16 +140,6 @@ instance Types.ULiftIterator.instIteratorCollectPartial {o} [Monad n] [Monad o] 
     IteratorCollectPartial (ULiftIterator α m n β lift) n o :=
   .defaultImplementation
 
-instance Types.ULiftIterator.instIteratorSize [Monad n] [Iterator α m β] [IteratorSize α m]
-    [Finite (ULiftIterator α m n β lift) n] :
-    IteratorSize (ULiftIterator α m n β lift) n where
-  size it := it.internalState.inner.size
-
-instance Types.ULiftIterator.instIteratorSizePartial [Monad n] [Iterator α m β]
-    [IteratorSizePartial α m] :
-    IteratorSizePartial (ULiftIterator α m n β lift) n where
-  size it := it.internalState.inner.allowNontermination.size
-
 /--
 Transforms an `m`-monadic iterator with values in `β` into an `n`-monadic iterator with
 values in `ULift β`. Requires a `MonadLift m (ULiftT n)` instance.
